src/Mail2/AtomicReadImpl.v
@@ -1,0 +1,235 @@
+Require Import POCS.
+Require Import String.
+Require Import MailboxAPI.
+Require Import FMapFacts.
+
+
+Instance key_elt_equiv : Equivalence (MailboxAPI.Dir.eq_key_elt (elt:=string)).
+Proof.
+  split; intro; intros.
+  - constructor; eauto.
+  - inversion H. constructor; eauto.
+  - inversion H. inversion H0. constructor; congruence.
+Qed.
+
+Hint Resolve key_elt_equiv.
+
+
+Module AtomicReader <: LayerImpl MailboxAPI AtomicMailboxAPI.
+
+  Definition deliver_core (m : string) :=
+    _ <- Op (MailboxAPI.Deliver m);
+    Ret tt.
+
+  Fixpoint read_list (l : list string) :=
+    match l with
+    | nil => Ret nil
+    | fn :: l' =>
+      m <- Op (MailboxAPI.Read fn);
+      rest <- read_list l';
+      Ret (m :: rest)
+    end.
+
+  Definition readall_core :=
+    l <- Op MailboxAPI.List;
+    read_list l.
+
+  Definition compile_op T (op : AtomicMailboxAPI.opT T) : proc _ T :=
+    match op with
+    | AtomicMailboxAPI.Deliver m => deliver_core m
+    | AtomicMailboxAPI.ReadAll => readall_core
+    end.
+
+  Ltac step_inv :=
+    match goal with
+    | H : MailboxAPI.step _ _ _ _ _ |- _ =>
+      inversion H; clear H; subst; repeat sigT_eq
+    | H : AtomicMailboxAPI.step _ _ _ _ _ |- _ =>
+      inversion H; clear H; subst; repeat sigT_eq
+    end; intuition idtac.
+
+  Hint Extern 1 (MailboxAPI.step _ _ _ _ _) => econstructor.
+  Hint Extern 1 (AtomicMailboxAPI.step _ _ _ _ _) => econstructor.
+
+  Module DirFacts := WFacts_fun String_as_OT MailboxAPI.Dir.
+
+  Lemma read_left_mover : forall fn,
+    left_mover_pred
+      MailboxAPI.step
+      (MailboxAPI.Read fn)
+      (fun s => MailboxAPI.Dir.In fn s).
+  Proof.
+    split.
+    - unfold enabled_stable, enabled_in; intros; repeat deex.
+      repeat step_inv; eauto.
+      destruct (fn0 == fn); subst; try congruence.
+      + exfalso. eapply H10. eexists. eauto.
+      + do 2 eexists; econstructor.
+        eapply MailboxAPI.Dir.add_2; eauto.
+    - intros; repeat step_inv; eauto; repeat deex.
+      destruct (fn0 == fn); subst; try congruence.
+      eapply MailboxAPI.Dir.add_3 in H5; eauto.
+  Qed.
+
+  Theorem deliver_atomic : forall `(rx : _ -> proc _ T) m,
+    trace_incl MailboxAPI.step
+      (Bind (compile_op (AtomicMailboxAPI.Deliver m)) rx)
+      (Bind (atomize compile_op (AtomicMailboxAPI.Deliver m)) rx).
+  Proof.
+    intros.
+    eapply trace_incl_atomize_ysa.
+    simpl.
+    unfold deliver_core.
+    eauto.
+  Qed.
+
+  Theorem readall_atomic : forall `(rx : _ -> proc _ T),
+    trace_incl MailboxAPI.step
+      (Bind (compile_op AtomicMailboxAPI.ReadAll) rx)
+      (Bind (atomize compile_op AtomicMailboxAPI.ReadAll) rx).
+  Proof.
+    intros.
+    eapply trace_incl_atomize_ysa.
+    simpl.
+    unfold readall_core.
+    eapply RightMoversDone.
+    eapply OneNonMover.
+    (* XXX need a state-based version... *)
+  Admitted.
+
+  Lemma read_list_exec : forall l s s' evs v tid,
+    List.Forall (fun fn => MailboxAPI.Dir.In fn s) l ->
+    atomic_exec MailboxAPI.step
+      (read_list l) tid
+      s v s' evs ->
+    s' = s /\ evs = nil /\
+    Forall2 (fun fn m => MailboxAPI.Dir.MapsTo fn m s) l v.
+  Proof.
+    induction l; intros.
+    - atomic_exec_inv.
+      eauto.
+    - atomic_exec_inv.
+      atomic_exec_inv.
+      atomic_exec_inv.
+      inversion H10; clear H10; subst; repeat sigT_eq.
+      inversion H; clear H; subst; eauto.
+      edestruct IHl; step_inv; eauto.
+      subst; eauto.
+  Qed.
+
+  Theorem my_compile_correct :
+    compile_correct compile_op MailboxAPI.step AtomicMailboxAPI.step.
+  Proof.
+    unfold compile_correct; intros.
+    destruct op.
+
+    + repeat atomic_exec_inv.
+      simpl; intuition eauto.
+      repeat step_inv; eauto.
+
+    + atomic_exec_inv.
+      eapply read_list_exec in H10.
+      {
+        atomic_exec_inv.
+        step_inv; subst; eauto.
+        econstructor.
+
+        assert (List.Forall (fun '(k, v) => MailboxAPI.Dir.MapsTo k v s1)
+                  (MailboxAPI.Dir.elements s1)).
+        {
+          eapply Forall_forall; intros.
+          destruct x.
+          eapply MailboxAPI.Dir.elements_2.
+          eapply In_InA; eauto.
+        }
+
+        generalize dependent (MailboxAPI.Dir.elements s1); intros.
+        generalize dependent v.
+        induction l; intros.
+        - inversion H2; eauto.
+        - inversion H2; clear H2; subst.
+          inversion H; clear H; subst.
+          specialize (IHl H4 _ H5); subst.
+          destruct a; simpl in *; f_equal.
+          eapply DirFacts.MapsTo_fun; eauto.
+      }
+
+      clear H10.
+      atomic_exec_inv.
+      step_inv.
+
+      eapply Forall_forall; intros.
+      eapply in_map_iff in H; deex.
+      destruct x0.
+      eapply DirFacts.elements_in_iff; eexists.
+      eapply In_InA; eauto.
+  Qed.
+
+  Theorem my_atomize_correct :
+    atomize_correct compile_op MailboxAPI.step.
+  Proof.
+    unfold atomize_correct; intros.
+    destruct op.
+    + rewrite deliver_atomic.
+      eapply trace_incl_bind_a.
+      eauto.
+    + rewrite readall_atomic.
+      eapply trace_incl_bind_a.
+      eauto.
+  Qed.
+
+  Hint Resolve my_compile_correct.
+  Hint Resolve my_atomize_correct.
+
+  Theorem all_traces_match :
+    forall ts1 ts2,
+      proc_match (Compile.compile_ok compile_op) ts1 ts2 ->
+      traces_match_ts MailboxAPI.step AtomicMailboxAPI.step ts1 ts2.
+  Proof.
+    intros.
+    eapply Compile.compile_traces_match_ts; eauto.
+  Qed.
+
+  Definition absR (s1 : MailboxAPI.State) (s2 : AtomicMailboxAPI.State) :=
+    s1 = s2.
+
+  Definition compile_ts := Compile.compile_ts compile_op.
+
+  Lemma read_list_no_atomics : forall l,
+    no_atomics (read_list l).
+  Proof.
+    induction l; simpl; eauto.
+  Qed.
+
+  Hint Resolve read_list_no_atomics.
+
+  Theorem compile_ts_no_atomics :
+    forall ts,
+      no_atomics_ts ts ->
+      no_atomics_ts (compile_ts ts).
+  Proof.
+    eapply Compile.compile_ts_no_atomics.
+    destruct op; compute; eauto.
+  Qed.
+
+  Theorem compile_traces_match :
+    forall ts2,
+      no_atomics_ts ts2 ->
+      traces_match_abs absR MailboxAPI.initP MailboxAPI.step AtomicMailboxAPI.step (compile_ts ts2) ts2.
+  Proof.
+    unfold traces_match_abs; intros.
+    rewrite H2 in *; clear H2.
+    eapply all_traces_match; eauto.
+    eapply Compile.compile_ts_ok; eauto.
+  Qed.
+
+  Theorem absInitP :
+    forall s1 s2,
+      MailboxAPI.initP s1 ->
+      absR s1 s2 ->
+      AtomicMailboxAPI.initP s2.
+  Proof.
+    eauto.
+  Qed.
+
+End AtomicReader.
