src/Mail2/MailboxAPI.v
@@ -1,0 +1,78 @@
+Require Import POCS.
+Require Import FMapInterface.
+Require Import FMapAVL.
+Require Import String.
+
+
+Module MailboxAPI <: Layer.
+
+  Module Dir := FMapAVL.Make(String_as_OT).
+
+  Definition mbox_contents := Dir.t string.
+
+  Inductive mbox_opT : Type -> Type :=
+  | Deliver : forall (m : string), mbox_opT unit
+  | List : mbox_opT (list string)
+  | Read : forall (fn : string), mbox_opT string
+  .
+
+  Definition opT := mbox_opT.
+  Definition State := mbox_contents.
+  Definition initP (s : State) := True.
+
+  Inductive xstep : forall T, opT T -> nat -> State -> T -> State -> Prop :=
+  | StepDeliver : forall m mbox tid fn,
+    ~ Dir.In fn mbox ->
+    xstep (Deliver m) tid
+      mbox
+      tt
+      (Dir.add fn m mbox)
+  | StepList : forall mbox tid,
+    xstep List tid
+      mbox
+      (map fst (Dir.elements mbox))
+      mbox
+  | StepRead : forall fn mbox tid m,
+    Dir.MapsTo fn m mbox ->
+    xstep (Read fn) tid
+      mbox
+      m
+      mbox
+  .
+
+  Definition step := xstep.
+
+End MailboxAPI.
+
+
+Module AtomicMailboxAPI <: Layer.
+
+  Module Dir := MailboxAPI.Dir.
+
+  Inductive atomic_mbox_opT : Type -> Type :=
+  | Deliver : forall (m : string), atomic_mbox_opT unit
+  | ReadAll : atomic_mbox_opT (list string)
+  .
+
+  Definition opT := atomic_mbox_opT.
+  Definition State := MailboxAPI.State.
+  Definition initP (s : State) := True.
+
+  Inductive xstep : forall T, opT T -> nat -> State -> T -> State -> Prop :=
+  | StepDeliver : forall m mbox tid fn,
+    ~ Dir.In fn mbox ->
+    xstep (Deliver m) tid
+      mbox
+      tt
+      (Dir.add fn m mbox)
+  | StepList : forall mbox tid r,
+    r = map snd (Dir.elements mbox) ->
+    xstep ReadAll tid
+      mbox
+      r
+      mbox
+  .
+
+  Definition step := xstep.
+
+End AtomicMailboxAPI.
